---
layout: default
title: "Algebraic Identities"
---

$$
(a + b)^2 = a^2 + 2ab + b^2
$$

$$
(a - b)^2 = a^2 - 2ab + b^2
$$

$$
a^2 + b^2 = (a + b)^2 - 2ab
$$

$$
a^2 - b^2 = (a + b)(a - b)
$$

$$
(a + b)^2 = (a - b)^2 + 4ab
$$

$$
(a - b)^2 = (a + b)^2 - 4ab
$$

$$
a^2 + b^2 = (a - b)^2 + 2ab
$$

$$
2(a^2 + b^2) = (a + b)^2 + (a - b)^2
$$

$$
4ab = (a + b)^2 - (a - b)^2
$$

$$
(a + b)^2 - (a - b)^2 = 4ab
$$

$$
(a + b)^2 + (a - b)^2 = 2(a^2 + b^2)
$$

$$
(a + b + c)^2 = a^2 + b^2 + c^2 + 2(ab + bc + ca)
$$

$$
(a + b - c)^2 = a^2 + b^2 + c^2 + 2(ab - bc - ca)
$$

$$
(a - b + c)^2 = a^2 + b^2 + c^2 - 2(ab - bc + ca)
$$

$$
(a - b - c)^2 = a^2 + b^2 + c^2 - 2(ab + bc + ca)
$$

$$
a^3 + b^3 = (a + b)(a^2 - ab + b^2)
$$

$$
a^3 - b^3 = (a - b)(a^2 + ab + b^2)
$$

$$
a^3 + b^3 = (a + b)^3 - 3ab(a + b)
$$

$$
a^3 - b^3 = (a - b)^3 + 3ab(a - b)
$$

$$
(x + a)(x + b) = x^2 + x(a + b) + ab
$$

$$
(x - a)(x - b) = x^2 - x(a + b) + ab
$$

$$
(x + a)(x - b) = x^2 + x(a - b) - ab
$$

$$
(x - a)(x + b) = x^2 + x(b - a) - ab
$$

$$
(a + b + c)^
